update definitions of System

ver2_qbft_Style/System.dfy
@@ -8,38 +8,79 @@ module M_System {
     import opened M_Replica
     import opened M_Adversary
 
-
+    /**
+     * Definition of a system state
+     * @param configuration -> infomations about system settings, such like node address, genesis block, etc.
+     * @param nodeStates -> a map storing node states, using node address as key
+     * @param adversary -> structure for Byzantine nodes
+     */
     datatype SystemState = SystemState(
         configuration : Configuration,
-        nodes : map<Address, ReplicaState>,
+        nodeStates : map<Address, ReplicaState>,
         adversary : Adversary
     )
 
+    /**
+     * Replicas not in adversary are considered as an honest node
+     * return `true` if and only if replica exists in the set of all nodes and not in the set of Byzantine nodes.
+     */
     predicate IsHonest(ss : SystemState, r : Address)
     {
-        r in ss.nodes.Keys - ss.adversary.nodes
+        r in ss.nodeStates.Keys - ss.adversary.byz_nodes
     }
 
+    /**
+     * Definition of initial state of system
+     */
     predicate SystemInit(ss : SystemState, c : Configuration)
     {
-        && (forall r | r in ss.nodes :: ReplicaInit(ss.nodes[r], r, c))
-        && AdversaryInit(ss.adversary, ss.nodes.Keys)
+        && (forall r | r in ss.nodeStates :: ReplicaInit(ss.nodeStates[r], r, c))
+        && AdversaryInit(ss.adversary, c)
     }
 
-    predicate SystemNextByOneReplica(ss : SystemState, ss' : SystemState, r : Address, outMsg : set<MsgWithRecipient>)
+
+    /**
+     * Definiton of system state transition triggered by a particular node
+     * @param ss -> current system state
+     * @param ss' -> next system state
+     * @param replica -> address of the node causing this state transition
+     * @param inMsg -> messages recieved by this node
+     * @param outMsg -> messages sent when state transition happens
+     */
+    predicate SystemNextByOneReplica(
+        ss : SystemState, 
+        ss' : SystemState, 
+        replica : Address, 
+        inMsg: multiset<MsgWithRecipient>,
+        outMsg : set<MsgWithRecipient>)
     {
+        && (forall mr:MsgWithRecipient | mr in inMsg :: mr.recipient == replica)
+        && var msgRecievedSingleSet := set mr:MsgWithRecipient | mr in inMsg :: mr.msg;
+        && replica in ss.nodeStates
+        && ss.nodeStates.Keys == ss'.nodeStates.Keys
         && (
-            if IsHonest(ss, r) then
-                ReplicaNext(ss.nodes[r], ss'.nodes[r], outMsg)
+            if IsHonest(ss, replica) then
+                && ss'.nodeStates == ss.nodeStates[replica := ss'.nodeStates[replica]]
+                && ss'.adversary == ss.adversary
+                && ReplicaNext(ss.nodeStates[replica], ss'.nodeStates[replica], outMsg)
             else
-                AdversaryNext(ss.adversary, ss'.adversary, outMsg)
+                && ss'.nodeStates == ss.nodeStates
+                && AdversaryNext(ss.adversary, msgRecievedSingleSet, ss'.adversary, outMsg)
         )
+        && ss'.configuration == ss.configuration
     }
 
+    /**
+     * Definition of transition state of system
+     * @param ss -> current system state
+     * @param ss' -> next system state
+     */
     ghost predicate SystemNext(ss : SystemState, ss' : SystemState)
     {
         || ss == ss'
-        || (exists r, msgRecievedByNodes
-                     :: SystemNextByOneReplica(ss, ss', r, msgRecievedByNodes))
+        || (exists replica,
+                   msgRecievedByNodes,
+                   msgSentByNodes
+                     :: SystemNextByOneReplica(ss, ss', replica, msgRecievedByNodes, msgSentByNodes))
     }
 }
